lunarlander_sl/ext2/BigStepContinuousEx.thy
@@ -1,0 +1,312 @@
+theory BigStepContinuousEx
+  imports BigStepContinuous
+begin
+
+subsection \<open>Examples\<close>
+
+definition X :: char where "X = CHR ''x''"
+definition Y :: char where "Y = CHR ''y''"
+definition Z :: char where "Z = CHR ''z''"
+definition ch1 :: cname where "ch1 = ''ch1''"
+definition ch2 :: cname where "ch2 = ''ch2''"
+
+subsubsection \<open>Example 1\<close>
+
+text \<open>
+  The program to be analyzed is:
+   x := 0; (ch!1; <x_dot = 2> |> dh?Y) \<squnion> (ch!2; <x_dot = 1> |> dh?Y)
+|| ch?Y; wait(Y); dh!0
+\<close>
+
+definition ex1a :: "'a proc" where
+  "ex1a = (X ::= (\<lambda>_. 0); IChoice
+      (Cm (ch1[!](\<lambda>_. 1)); Interrupt (ODE ((\<lambda>_ _. 0)(X := (\<lambda>_. 2)))) (\<lambda>_. True)
+                                     [(ch2[?]Y, Skip)])
+      (Cm (ch1[!](\<lambda>_. 2)); Interrupt (ODE ((\<lambda>_ _. 0)(X := (\<lambda>_. 1)))) (\<lambda>_. True)
+                                     [(ch2[?]Y, Skip)]))"
+
+lemma ex1a_ode:
+  "spec_of (Interrupt (ODE ((\<lambda>_ _. 0)(X := \<lambda>_. 2))) (\<lambda>_. True) [(ch2[?]Y, Skip)])
+           (interrupt_solInf_c (\<lambda>s0 t. (rpart s0)(X := val s0 X + 2 * t))
+                               ({}, {ch2})
+                               [InSpec2 ch2 (\<lambda>d v s. init (upd (upd s X (val s X + 2 * d)) Y v))])"
+proof -
+  have 1: "paramODEsolInf (ODE ((\<lambda>_ _. 0)(X := \<lambda>_. 2)))
+                          (\<lambda>s0 t. (rpart s0)(X := val s0 X + 2 * t))"
+    unfolding paramODEsolInf_def apply clarify
+    subgoal for s
+      apply (rule conjI)
+      subgoal apply (cases s)
+        by (auto simp add: rpart.simps val.simps)
+      unfolding ODEsolInf_def solves_ode_def has_vderiv_on_def
+      apply auto
+      apply (rule exI[where x="1"])
+      apply auto
+      apply (rule has_vector_derivative_projI)
+      apply (auto simp add: state2vec_def)
+      apply (rule has_vector_derivative_eq_rhs)
+       apply (auto intro!: derivative_intros)[1]
+      by simp
+    done
+  have 2: "local_lipschitz {- 1<..} UNIV (\<lambda>t v. ODE2Vec (ODE ((\<lambda>_ _. 0)(X := \<lambda>_. 2))) (vec2state v))"
+  proof -
+    have eq: "(\<chi> a. (if a = X then \<lambda>_. 2 else (\<lambda>_. 0)) (($) v)) = (\<chi> a. if a = X then 2 else 0)" for v::vec
+      by auto
+    show ?thesis
+      unfolding fun_upd_def vec2state_def
+      apply (auto simp add: state2vec_def eq)
+      by (rule local_lipschitz_constI)
+  qed
+  let ?specs = "[InSpec ch2 Y init]"
+  show ?thesis
+    apply (rule spec_of_post)
+     apply (rule spec_of_interrupt_inf_unique[where specs="?specs"])
+        apply (rule 1) apply (rule 2)
+      apply auto apply (rule spec_of_es.intros)
+     apply (rule spec_of_skip)
+    subgoal for s0
+      apply (rule interrupt_solInf_mono)
+       apply auto
+      apply (intro spec2_entails.intros)
+      subgoal for d v s0
+        apply (cases s0) apply (auto simp add: updr.simps rpart.simps val.simps upd.simps)
+        by (rule entails_triv)
+      done
+    done
+qed
+
+lemma ex1a_ode2:
+  "spec_of (Interrupt (ODE ((\<lambda>_ _. 0)(X := (\<lambda>_. 1)))) (\<lambda>_. True)
+                      [(dh[?]Y, Skip)])
+           (interrupt_solInf_c (\<lambda>s0 t. (rpart s0)(X := val s0 X + t))
+                               ({}, {dh})
+                               [InSpec2 dh (\<lambda>d v s. init (upd (upd s X (val s X + d)) Y v))])"
+proof -
+  have 1: "paramODEsolInf (ODE ((\<lambda>_ _. 0)(X := \<lambda>_. 1)))
+                       (\<lambda>s0 t. (rpart s0)(X := val s0 X + t))"
+    unfolding paramODEsolInf_def apply clarify
+    subgoal for s
+      apply (rule conjI)
+      subgoal apply (cases s)
+        by (auto simp add: rpart.simps val.simps)
+      unfolding ODEsolInf_def solves_ode_def has_vderiv_on_def
+      apply auto
+      apply (rule exI[where x="1"])
+      apply auto
+      apply (rule has_vector_derivative_projI)
+      apply (auto simp add: state2vec_def)
+      apply (rule has_vector_derivative_eq_rhs)
+       apply (auto intro!: derivative_intros)[1]
+      by simp
+    done
+  have 2: "local_lipschitz {- 1<..} UNIV (\<lambda>t v. ODE2Vec (ODE ((\<lambda>_ _. 0)(X := \<lambda>_. 1))) (vec2state v))"
+  proof -
+    have eq: "(\<chi> a. (if a = X then \<lambda>_. 1 else (\<lambda>_. 0)) (($) v)) = (\<chi> a. if a = X then 1 else 0)" for v::vec
+      by auto
+    show ?thesis
+      unfolding fun_upd_def vec2state_def
+      apply (auto simp add: state2vec_def eq)
+      by (rule local_lipschitz_constI)
+  qed
+  let ?specs = "[InSpec dh Y init]"
+  show ?thesis
+    apply (rule spec_of_post)
+     apply (rule spec_of_interrupt_inf_unique[where specs="?specs"])
+        apply (rule 1) apply (rule 2)
+      apply auto apply (rule spec_of_es.intros)
+     apply (rule spec_of_skip)
+    subgoal for s0
+      apply (rule interrupt_solInf_mono)
+       apply auto
+      apply (intro spec2_entails.intros)
+      subgoal for d v s0
+        apply (cases s0) apply (auto simp add: updr.simps rpart.simps val.simps upd.simps)
+        by (rule entails_triv)
+      done
+    done
+qed
+
+lemma ex1a_sp:
+  "spec_of ex1a
+     ((wait_out_c ch1 (\<lambda>_. 1)
+        (\<lambda>d. interrupt_solInf_c (\<lambda>s0 t. (rpart s0)(X := val s0 X + 2 * t)) ({}, {ch2})
+                                [InSpec2 ch2 (\<lambda>d v s. init (upd (upd s X (val s X + 2 * d)) Y v))]) \<or>\<^sub>a
+       wait_out_c ch1 (\<lambda>_. 2)
+        (\<lambda>d. interrupt_solInf_c (\<lambda>s0 t. (rpart s0)(X := val s0 X + t)) ({}, {ch2})
+                                [InSpec2 ch2 (\<lambda>d v s. init (upd (upd s X (val s X + d)) Y v))]))
+      {{X := (\<lambda>_. 0)}})"
+  unfolding ex1a_def
+  apply (rule spec_of_post)
+   apply (rule Valid_assign_sp)
+   apply (rule spec_of_ichoice)
+    apply (rule Valid_send_sp)
+    apply (rule ex1a_ode)
+  apply (rule Valid_send_sp)
+   apply (rule ex1a_ode2)
+  apply auto by (rule entails_triv)
+
+definition ex1b :: "'a proc" where
+  "ex1b = (Cm (ch2[?]Y); Wait (\<lambda>s. val s Y); Cm (ch2[!](\<lambda>_. 0)))"
+
+lemma ex1b_sp:
+  "spec_of ex1b
+           (wait_in_c ch2 (\<lambda>d v.
+              wait_c (\<lambda>s. val s Y) (
+                wait_out_c ch2 (\<lambda>_. 0) (\<lambda>d. init)) {{Y := (\<lambda>_. v)}}))"
+  unfolding ex1b_def
+  apply (rule spec_of_post)
+  apply (rule Valid_receive_sp)
+   apply (rule Valid_wait_sp)
+   apply (rule spec_of_send)
+  apply auto by (rule entails_triv)
+
+datatype 'a comm_specg2 =
+  InSpecg2 cname "real \<Rightarrow> real \<Rightarrow> 'a gassn2"
+| OutSpecg2 cname pname "'a eexp" "real \<Rightarrow> 'a gassn2"
+
+text \<open>Mapping from path on a single state to path on general states\<close>
+definition single_path :: "pname \<Rightarrow> ('a estate \<Rightarrow> real \<Rightarrow> state) \<Rightarrow> 'a gstate \<Rightarrow> real \<Rightarrow> 'a gstate" where
+  "single_path pn p gs t = gs (pn \<mapsto> updr (the (gs pn)) (p (the (gs pn)) t))"
+
+lemma single_path_State:
+  "single_path pn p (State pn s) t = State pn (updr s (p s t))"
+  unfolding single_path_def
+  by (auto simp add: State_def)
+
+text \<open>Mapping from specification on single state to specification
+  on general states.
+\<close>
+fun gassn_of :: "pname \<Rightarrow> 'a comm_spec2 \<Rightarrow> 'a comm_specg2" where
+  "gassn_of pn (InSpec2 ch Q) = InSpecg2 ch (\<lambda>d v. single_assn pn (Q d v))"
+| "gassn_of pn (OutSpec2 ch e Q) = OutSpecg2 ch pn e (\<lambda>d. single_assn pn (Q d))"
+
+inductive interrupt_solInf_cg :: "('a gstate \<Rightarrow> real \<Rightarrow> 'a gstate) \<Rightarrow> rdy_info \<Rightarrow>
+  'a comm_specg2 list \<Rightarrow> 'a gassn2" where
+  "i < length specs \<Longrightarrow> specs ! i = InSpecg2 ch Q \<Longrightarrow>
+   Q 0 v gs0 gs tr \<Longrightarrow> interrupt_solInf_cg p rdy specs gs0 gs (InBlockP ch v # tr)"
+| "i < length specs \<Longrightarrow> specs ! i = InSpecg2 ch Q \<Longrightarrow>
+   0 < d \<Longrightarrow> Q d v gs0 gs tr \<Longrightarrow>
+   interrupt_solInf_cg p rdy specs gs0 gs (WaitBlockP d (\<lambda>\<tau>\<in>{0..d}. p gs0 \<tau>) rdy # InBlockP ch v # tr)"
+| "i < length specs \<Longrightarrow> specs ! i = OutSpecg2 ch pn e Q \<Longrightarrow>
+   v = e (the (gs0 pn)) \<Longrightarrow>
+   Q 0 gs0 gs tr \<Longrightarrow> interrupt_solInf_cg p rdy specs gs0 gs (OutBlockP ch v # tr)"
+| "i < length specs \<Longrightarrow> specs ! i = OutSpecg2 ch pn e Q \<Longrightarrow>
+   0 < d \<Longrightarrow> Q d gs0 gs tr \<Longrightarrow>
+   v = e (the (p gs0 d pn)) \<Longrightarrow>
+   interrupt_solInf_cg p rdy specs gs0 gs (WaitBlockP d (\<lambda>\<tau>\<in>{0..d}. p gs0 \<tau>) rdy # OutBlockP ch v # tr)"
+
+lemma single_assn_interrupt_solInf:
+  "single_assn pn (interrupt_solInf_c p rdy specs) =
+   interrupt_solInf_cg (single_path pn p) rdy (map (gassn_of pn) specs)"
+  apply (rule ext) apply (rule ext) apply (rule ext)
+  subgoal for s0 s tr
+    apply (rule iffI)
+    subgoal apply (elim single_assn.cases) apply auto
+      subgoal for s0' s' tr'
+        apply (elim interrupt_solInf_c.cases) apply auto
+        subgoal for i ch Q v tr'' a b
+          apply (rule interrupt_solInf_cg.intros(1)[of i _ _ "(\<lambda>d v. single_assn pn (Q d v))"])
+          by (auto intro: single_assn.intros)
+        subgoal premises pre for i ch Q d v tr'' a b
+        proof -
+          have 1: "(\<lambda>\<tau>\<in>{0..d}. State pn (if 0 \<le> \<tau> \<and> \<tau> \<le> d then updr s0' (p s0' \<tau>) else undefined)) =
+                   (\<lambda>\<tau>\<in>{0..d}. single_path pn p (State pn s0') \<tau>)"
+            unfolding single_path_State by auto
+          show ?thesis
+            unfolding 1
+            apply (rule interrupt_solInf_cg.intros(2)[of i _ _ "(\<lambda>d v. single_assn pn (Q d v))"])
+            using pre by (auto intro: single_assn.intros)
+        qed
+        subgoal for i ch e Q tr'' a b
+          apply (rule interrupt_solInf_cg.intros(3)[of i _ _ pn e "(\<lambda>d. single_assn pn (Q d))" ])
+          by (auto intro: single_assn.intros)
+        subgoal premises pre for i ch e Q d tr'' a b
+        proof -
+          have 1: "(\<lambda>\<tau>\<in>{0..d}. State pn (if 0 \<le> \<tau> \<and> \<tau> \<le> d then updr s0' (p s0' \<tau>) else undefined)) =
+                   (\<lambda>\<tau>\<in>{0..d}. single_path pn p (State pn s0') \<tau>)"
+            unfolding single_path_State by auto
+          show ?thesis
+            unfolding 1
+            apply (rule interrupt_solInf_cg.intros(4)[of i _ _ pn e "(\<lambda>d. single_assn pn (Q d))"])
+            using pre by (auto intro: single_assn.intros simp: single_path_State)
+        qed
+        done
+      done
+    subgoal apply (elim interrupt_solInf_cg.cases) apply auto
+      subgoal for i ch Q v tr' a b
+        apply (cases "specs ! i") apply auto
+        apply (elim single_assn.cases) apply auto
+        subgoal for Q' s0' s' tr''
+          apply (subst ptrace_of.simps[symmetric])
+          apply (rule single_assn.intros)
+          apply (rule interrupt_solInf_c.intros(1)[of i _ _ Q']) by auto
+        done
+      subgoal for i ch Q d v tr' a b
+        apply (cases "specs ! i") apply auto
+        apply (elim single_assn.cases) apply auto
+        subgoal for Q' s0'' s' tr''
+          unfolding single_path_State
+          apply (subst ptrace_of.simps(2)[symmetric])
+          apply (subst ptrace_of_simp3[symmetric])
+          apply (rule single_assn.intros)
+          apply (rule interrupt_solInf_c.intros(2)[of i _ _ Q']) by auto
+        done
+      subgoal for i ch pn e Q tr' a b
+        apply (cases "specs ! i") apply auto
+        apply (elim single_assn.cases) apply auto
+        subgoal for Q' s0'' s' tr''
+          apply (subst ptrace_of.simps[symmetric])
+          apply (rule single_assn.intros)
+          apply (rule interrupt_solInf_c.intros(3)[of i _ _ _ Q']) by auto
+        done
+      subgoal for i ch pn e Q d tr' a b
+        apply (cases "specs ! i") apply auto
+        apply (elim single_assn.cases) apply auto
+        subgoal for Q' s0'' s' tr''
+          unfolding single_path_State
+          apply (subst ptrace_of.simps[symmetric])
+          apply (subst ptrace_of_simp3[symmetric])
+          apply (rule single_assn.intros)
+          apply (rule interrupt_solInf_c.intros(4)[of i _ _ _ Q']) by auto
+        done
+      done
+    done
+  done
+
+definition disj_gassn :: "'a gassn2 \<Rightarrow> 'a gassn2 \<Rightarrow> 'a gassn2" (infixr "\<or>\<^sub>g" 35) where
+  "(P \<or>\<^sub>g Q) gs0 = (\<lambda>gs tr. P gs0 gs tr \<or> Q gs0 gs tr)"
+
+lemma single_assn_disj:
+  "single_assn pn (P \<or>\<^sub>a Q) = (single_assn pn P \<or>\<^sub>g single_assn pn Q)"
+  apply (rule ext) apply (rule ext) apply (rule ext)
+  subgoal for s0 s tr
+    apply (rule iffI)
+    subgoal apply (elim single_assn.cases) apply auto
+      subgoal for s0' s' tr'
+        unfolding disj_gassn_def disj_assn2_def
+        by (auto intro: single_assn.intros)
+      done
+    subgoal unfolding disj_gassn_def disj_assn2_def
+      apply (elim disjE single_assn.cases)
+      by (auto intro: single_assn.intros)
+    done
+  done
+
+lemma ex1b:
+  "spec_of_global
+    (Parallel (Single ''a'' ex1a)
+              {ch1, ch2}
+              (Single ''b'' ex1b))
+   Q"
+  (* Stage 1: merge ex1a_sp and ex1b_sp *)
+  apply (rule spec_of_global_post)
+   apply (rule spec_of_parallel)
+      apply (rule spec_of_single) apply (rule ex1a_sp)
+     apply (rule spec_of_single) apply (rule ex1b_sp)
+  (* Stage 2: rewrite the assertions *)
+    apply auto subgoal for s0
+    apply (auto simp: single_assn_wait_in single_assn_wait single_assn_wait_out
+                      single_assn_init single_assn_interrupt_solInf single_assn_disj updg_subst2)
+
+
+end
